Rename parser implementations

LL1/Parser.v
@@ -591,10 +591,11 @@ Fixpoint parse2 (tbl     : parse_table)
   - eapply (pf_lt_args _ _ Htri Hsa Hgamma Htri' Htri''); eauto.
 Defined.
 
-Program Fixpoint parse3 (tbl     : parse_table)
-        (tri     : list string * list nonterminal * sym_arg)
-        (a : Acc triple_lt (meas tbl tri))
-        {struct a}
+(* Fuel-less LL(1) parser with termination proof "inlined" *)
+Fixpoint parse3 (tbl     : parse_table)
+         (tri     : list string * list nonterminal * sym_arg)
+         (a : Acc triple_lt (meas tbl tri))
+         {struct a}
   : sum parse_failure
         (sum (list tree * {tri' | triple_le (meas tbl tri') (meas tbl tri)})
              (tree      * {tri' | triple_lt (meas tbl tri') (meas tbl tri)})) :=
@@ -650,66 +651,6 @@ Program Fixpoint parse3 (tbl     : parse_table)
                 end eq_refl
   end eq_refl.
 
-(* to do : some of the match annotations might actually be unnecessary *)
-Fixpoint parse_no_fuel (tbl     : parse_table)
-         (tri     : list string * list nonterminal * sym_arg)
-         (a : Acc triple_lt (meas tbl tri))
-         {struct a}
-  : sum parse_failure
-        (sum (list tree * {tri' | triple_le (meas tbl tri') (meas tbl tri)})
-             (tree      * {tri' | triple_lt (meas tbl tri') (meas tbl tri)})) :=
-  match tri as tri' return tri = tri' -> _ with
-  | (word, vis, sa) =>
-    fun Htri => match sa as sa' return sa = sa' -> _ with
-                | F_arg sym =>
-                  (* morally, a call to parse *)
-                  fun Hsa => match sym with
-                             | T y  => match word as w return word = w -> _ with
-                                       | [] => fun _ => inl (Mismatch "error message" word)
-                                       | token :: word' =>
-                                         if beqString y token then
-                                           fun Hword =>
-                                             inr (inr (Leaf y, exist _ (word', nil, sa) (tail_lt_word tbl _ _ Htri Hword)))
-                                         else
-                                           fun _ => inl (Mismatch "error message" word)
-                                       end eq_refl
-                             | NT x =>
-                               match List.in_dec NT_as_DT.eq_dec x vis with
-                               | left _ => inl (LeftRec (x :: vis))
-                               | right Hnin => 
-                                 match pt_lookup x (peek word) tbl as H return  pt_lookup x (peek word) tbl = H -> _ with
-                                 | None => fun _ => inl (Mismatch "error message" word)
-                                 | Some gamma =>
-                                   fun Hlk => match parse_no_fuel tbl (word, x :: vis, G_arg gamma) (acc_vis_add tbl x Htri Hsa Hnin Hlk a) with
-                                              | inl pf => inl pf
-                                              | inr (inr (_, _)) => inl Error
-                                              | inr (inl (sts, exist _ tri' Htri')) =>
-                                                inr (inr (Node x sts, exist _ tri' (vis_lt_add tri' Htri Hnin Hlk Htri')))
-                                              end
-                                 end eq_refl
-                               end
-                             end
-                | G_arg gamma =>
-                  (* a call to parseForest *)
-                  fun Hsa => match gamma as g return gamma = g -> _ with
-                             | nil =>
-                               fun _ => inr (inl (nil, exist _ (word, vis, sa) (triple_le_refl tbl Htri)))
-                             | sym :: gamma' =>
-                               fun Hgamma => match parse_no_fuel tbl (word, vis, F_arg sym) (if_acc_gamma_then_acc_sym tbl a Htri Hsa Hgamma) with
-                                             | inl pf => inl pf
-                                             | inr (inl (_, _)) => inl Error
-                                             | inr (inr (lSib, exist _ tri' Htri')) =>
-                                               match parse_no_fuel tbl tri' (acc_triple_lt_trans tri' a Htri Hsa Hgamma Htri') with
-                                               | inl pf => inl pf
-                                               | inr (inr (_, _)) => inl Error
-                                               | inr (inl (rSibs, exist _ tri'' Htri'')) =>
-                                                 inr (inl (lSib :: rSibs, exist _ tri'' (pf_lt_args _ _ Htri Hsa Hgamma Htri' Htri'')))
-                                               end
-                                             end
-                             end eq_refl
-                end eq_refl
-  end eq_refl.
-
 Definition isLeft (A B : Type) (e : sum A B) : bool :=
   match e with
   | inl _ => true
@@ -725,7 +666,7 @@ Lemma sym_ret_inr :
          (vis : list nonterminal)
          (sa : sym_arg)
          e,
-    parse_no_fuel' tbl (word, vis, sa) (triple_lt_wf (meas tbl (word, vis, sa))) = inr e
+    parse3 tbl (word, vis, sa) (triple_lt_wf (meas tbl (word, vis, sa))) = inr e
     -> forall (sym : symbol),
       sa = F_arg sym
       -> isRight e = true.
@@ -736,7 +677,8 @@ Proof.
   - simpl in *.
     destruct word.
     + simpl in *.
-      unfold parse_no_fuel' in *.
+      unfold parse3 in *.
+      cbv in H.
 Abort.
 
 
